src/HOL/Auth/CertifiedEmail.thy
@@ -1,0 +1,522 @@
+(*  Title:      HOL/Auth/CertifiedEmail
+    ID:         $Id$
+    Author:     Giampaolo Bella, Christiano Longo and Lawrence C Paulson
+
+The certified electronic mail protocol by Abadi et al.
+*)
+
+theory CertifiedEmail = Public:
+
+syntax
+  TTP        :: agent
+  RPwd       :: "agent => key"
+  TTPDecKey  :: key
+  TTPEncKey  :: key
+  TTPSigKey  :: key
+  TTPVerKey  :: key
+
+translations
+  "TTP"   == "Server"
+  "RPwd"  == "shrK"
+  "TTPDecKey" == "priEK Server"
+  "TTPEncKey" == "pubEK Server" 
+  "TTPSigKey" == "priSK Server"
+  "TTPVerKey" == "pubSK Server" 
+
+ 
+(*FIXME: the four options should be represented by pairs of 0 or 1.
+  Right now only BothAuth is modelled.*)
+consts
+  NoAuth   :: nat
+  TTPAuth  :: nat
+  SAuth    :: nat
+  BothAuth :: nat
+
+text{*We formalize a fixed way of computing responses.  Could be better.*}
+constdefs
+  "response"    :: "agent => agent => nat => msg"
+   "response S R q == Hash {|Agent S, Key (shrK R), Nonce q|}"
+
+
+consts  certified_mail   :: "event list set"
+inductive "certified_mail"
+  intros 
+
+Nil: --{*The empty trace*}
+     "[] \<in> certified_mail"
+
+Fake: --{*The Spy may say anything he can say.  The sender field is correct,
+          but agents don't use that information.*}
+      "[| evsf \<in> certified_mail; X \<in> synth(analz(knows Spy evsf))|] 
+       ==> Says Spy B X #evsf \<in> certified_mail"
+
+FakeSSL: --{*The Spy may open SSL sessions with TTP, who is the only agent
+    equipped with the necessary credentials to serve as an SSL server.*}
+	 "[| evsfssl \<in> certified_mail; X \<in> synth(analz(knows Spy evsfssl))|]
+          ==> Notes TTP {|Agent Spy, Agent TTP, X|} # evsfssl \<in> certified_mail"
+
+CM1: --{*The sender approaches the recipient.  The message is a number.*}
+"[|evs1 \<in> certified_mail;
+   Key K \<notin> used evs1;
+   K \<in> symKeys;
+   Nonce q \<notin> used evs1;
+   hs = Hash {|Number cleartext, Nonce q, response S R q, Crypt K (Number m)|};
+   S2TTP = Crypt TTPEncKey {|Agent S, Number BothAuth, Key K, Agent R, hs|}|]
+ ==> Says S R {|Agent S, Agent TTP, Crypt K (Number m), Number BothAuth, 
+                Number cleartext, Nonce q, S2TTP|} # evs1 
+       \<in> certified_mail"
+
+CM2: --{*The recipient records @{term S2TTP'} while transmitting it and her
+     password to @{term TTP} over an SSL channel.*}
+"[|evs2 \<in> certified_mail;
+   Gets R {|Agent S, Agent TTP, em', Number BothAuth, Number cleartext', 
+            Nonce q', S2TTP'|} \<in> set evs2;
+   TTP \<noteq> R;  
+   hr = Hash {|Number cleartext', Nonce q', response S R q', em'|} |]
+ ==> 
+  Notes TTP {|Agent R, Agent TTP, S2TTP', Key(RPwd R), hr|} # evs2
+     \<in> certified_mail"
+
+CM3: --{*@{term TTP} simultaneously reveals the key to the recipient and gives
+         a receipt to the sender.  The SSL channel does not authenticate 
+         the client (@{term R'}), but @{term TTP} accepts the message only 
+         if the given password is that of the claimed sender, @{term R'}.
+         He replies over the established SSL channel.*}
+ "[|evs3 \<in> certified_mail;
+    Notes TTP {|Agent R', Agent TTP, S2TTP'', Key(RPwd R'), hr'|} \<in> set evs3;
+    S2TTP'' = Crypt TTPEncKey 
+                     {|Agent S, Number BothAuth, Key k', Agent R', hs'|};
+    TTP \<noteq> R';  hs' = hr';  k' \<in> symKeys|]
+ ==> 
+  Notes R' {|Agent TTP, Agent R', Key k', hr'|} # 
+  Says TTP S (Crypt TTPSigKey S2TTP'') # evs3 \<in> certified_mail"
+
+Reception:
+ "[|evsr \<in> certified_mail; Says A B X \<in> set evsr|]
+  ==> Gets B X#evsr \<in> certified_mail"
+
+
+axioms
+  (*Unlike the corresponding property of nonces, this cannot be proved.
+    We have infinitely many agents and there is nothing to stop their
+    long-term keys from exhausting all the natural numbers.  The axiom
+    assumes that their keys are dispersed so as to leave room for infinitely
+    many fresh session keys.  We could, alternatively, restrict agents to
+    an unspecified finite number.  TOO STRONG.  REPLACE "used evs" BY
+    used []*)
+  Key_supply_ax:  "finite KK ==> \<exists>K\<in>symKeys. K \<notin> KK & Key K \<notin> used evs"
+
+
+lemma Key_supply1: "\<exists>K\<in>symKeys. Key K \<notin> used evs"
+by (rule Finites.emptyI [THEN Key_supply_ax, THEN bexE], blast)
+
+(*A "possibility property": there are traces that reach the end*)
+lemma "\<exists>S2TTP. \<exists>evs \<in> certified_mail.
+           Says TTP S (Crypt TTPSigKey S2TTP) \<in> set evs"
+apply (rule bexE [OF Key_supply1]) 
+apply (intro exI bexI)
+apply (rule_tac [2] certified_mail.Nil
+                    [THEN certified_mail.CM1, THEN certified_mail.Reception,
+                     THEN certified_mail.CM2, 
+                     THEN certified_mail.CM3], possibility, possibility) 
+apply auto 
+done
+
+
+lemma Gets_imp_Says:
+ "[| Gets B X \<in> set evs; evs \<in> certified_mail |] ==> \<exists>A. Says A B X \<in> set evs"
+apply (erule rev_mp)
+apply (erule certified_mail.induct, auto)
+done
+
+
+lemma Gets_imp_parts_knows_Spy:
+     "[|Gets A X \<in> set evs; evs \<in> certified_mail|] ==> X \<in> parts(spies evs)"
+apply (drule Gets_imp_Says, simp)
+apply (blast dest: Says_imp_knows_Spy parts.Inj) 
+done
+
+lemma CM2_S2TTP_analz_knows_Spy:
+ "[|Gets R {|Agent A, Agent B, em, Number AO, Number cleartext, 
+              Nonce q, S2TTP|} \<in> set evs;
+    evs \<in> certified_mail|] 
+  ==> S2TTP \<in> analz(knows Spy evs)"
+apply (drule Gets_imp_Says, simp) 
+apply (blast dest: Says_imp_knows_Spy analz.Inj) 
+done
+
+lemmas CM2_S2TTP_parts_knows_Spy = 
+    CM2_S2TTP_analz_knows_Spy [THEN analz_subset_parts [THEN subsetD]]
+
+lemma hr_form_lemma [rule_format]:
+ "evs \<in> certified_mail
+  ==> hr \<notin> synth (analz (knows Spy evs)) --> 
+      (\<forall>S2TTP. Notes TTP {|Agent R, Agent TTP, S2TTP, pwd, hr|}
+          \<in> set evs --> 
+      (\<exists>clt q S em. hr = Hash {|Number clt, Nonce q, response S R q, em|}))"
+apply (erule certified_mail.induct)
+apply (synth_analz_mono_contra, simp_all, blast+)
+done 
+
+text{*Cannot strengthen the first disjunct to @{term "R\<noteq>Spy"} because
+the fakessl rule allows Spy to spoof the sender's name.  Maybe can
+strengthen the second disjunct with @{term "R\<noteq>Spy"}.*}
+lemma hr_form:
+ "[|Notes TTP {|Agent R, Agent TTP, S2TTP, pwd, hr|} \<in> set evs;
+    evs \<in> certified_mail|]
+  ==> hr \<in> synth (analz (knows Spy evs)) | 
+      (\<exists>clt q S em. hr = Hash {|Number clt, Nonce q, response S R q, em|})"
+by (blast intro: hr_form_lemma) 
+
+lemma Spy_dont_know_private_keys [rule_format]:
+    "evs \<in> certified_mail
+     ==> Key (privateKey b A) \<in> parts (spies evs) --> A \<in> bad"
+apply (erule certified_mail.induct, simp_all)
+txt{*Fake*}
+apply (blast dest: Fake_parts_insert[THEN subsetD]
+                   analz_subset_parts[THEN subsetD])
+txt{*Message 1*}
+apply blast  
+txt{*Message 3*}
+apply (frule_tac hr_form, assumption)
+apply (elim disjE exE) 
+apply (simp_all add: parts_insert2) 
+ apply (force dest!: parts_insert_subset_Un[THEN [2] rev_subsetD] 
+                     analz_subset_parts[THEN subsetD], blast) 
+done
+
+lemma Spy_know_private_keys_iff [simp]:
+    "evs \<in> certified_mail
+     ==> (Key (privateKey b A) \<in> parts (spies evs)) = (A \<in> bad)"
+by (blast intro: Spy_dont_know_private_keys parts.Inj)
+
+
+lemma CM3_k_parts_knows_Spy:
+ "[| evs \<in> certified_mail;
+     Notes TTP {|Agent A, Agent TTP,
+                 Crypt TTPEncKey {|Agent S, Number AO, Key K, 
+                 Agent R, hs|}, Key (RPwd R), hs|} \<in> set evs|]
+  ==> Key K \<in> parts(spies evs)"
+apply (rotate_tac 1)
+apply (erule rev_mp)
+apply (erule certified_mail.induct, simp_all)
+   apply (blast  intro:parts_insertI)
+txt{*Fake SSL*}
+apply (blast dest: analz_subset_parts[THEN subsetD] parts.Body) 
+txt{*Message 2*}
+apply (blast dest!: Says_imp_knows_Spy [THEN parts.Inj] Gets_imp_Says
+             elim!: knows_Spy_partsEs)
+txt{*Message 3*}
+apply (frule_tac hr_form, assumption)
+apply (elim disjE exE) 
+apply (simp_all add: parts_insert2)
+apply (blast intro: subsetD [OF parts_mono [OF Set.subset_insertI]])  
+done
+
+lemma Spy_dont_know_RPwd [rule_format]:
+    "evs \<in> certified_mail ==> Key (RPwd A) \<in> parts(spies evs) --> A \<in> bad"
+apply (erule certified_mail.induct, simp_all) 
+txt{*Fake*}
+apply (blast dest: Fake_parts_insert[THEN subsetD]
+                   analz_subset_parts[THEN subsetD])
+txt{*Message 1*}
+apply blast  
+txt{*Message 3*}
+apply (frule CM3_k_parts_knows_Spy, assumption)
+apply (frule_tac hr_form, assumption)
+apply (elim disjE exE) 
+apply (simp_all add: parts_insert2) 
+apply (force dest!: parts_insert_subset_Un[THEN [2] rev_subsetD]
+                    analz_subset_parts[THEN subsetD])
+done
+
+
+lemma Spy_know_RPwd_iff [simp]:
+    "evs \<in> certified_mail ==> (Key (RPwd A) \<in> parts(knows Spy evs)) = (A\<in>bad)"
+by (auto simp add: Spy_dont_know_RPwd) 
+
+lemma Spy_analz_RPwd_iff [simp]:
+    "evs \<in> certified_mail ==> (Key (RPwd A) \<in> analz(knows Spy evs)) = (A\<in>bad)"
+by (auto simp add: Spy_dont_know_RPwd [OF _ analz_subset_parts[THEN subsetD]]) 
+
+
+text{*Unused, but a guarantee of sorts*}
+theorem CertAutenticity:
+     "[|Crypt TTPSigKey X \<in> parts (spies evs); evs \<in> certified_mail|] 
+      ==> \<exists>A. Says TTP A (Crypt TTPSigKey X) \<in> set evs"
+apply (erule rev_mp)
+apply (erule certified_mail.induct, simp_all) 
+txt{*Fake*}
+apply (blast dest: Spy_dont_know_private_keys Fake_parts_insert[THEN subsetD]
+                   analz_subset_parts[THEN subsetD])
+txt{*Message 1*}
+apply blast 
+txt{*Message 3*}
+apply (frule_tac hr_form, assumption)
+apply (elim disjE exE) 
+apply (simp_all add: parts_insert2) 
+apply (force dest!: parts_insert_subset_Un[THEN [2] rev_subsetD]
+                    analz_subset_parts[THEN subsetD], blast) 
+done
+
+
+lemma Spy_dont_know_TTPDecKey [simp]:
+     "evs \<in> certified_mail ==> Key TTPDecKey \<notin> parts(knows Spy evs)"
+by auto
+
+lemma Spy_dont_know_TTPDecKey_analz [simp]:
+     "evs \<in> certified_mail ==> Key TTPDecKey \<notin> analz(knows Spy evs)" 
+by (force dest!: analz_subset_parts[THEN subsetD])
+
+
+lemma Spy_knows_TTPVerKey [simp]:
+     "Key (invKey TTPSigKey) \<in> analz(knows Spy evs)"
+by simp
+
+
+subsection{*Proving Confidentiality Results*}
+
+lemma analz_image_freshK [rule_format]:
+ "evs \<in> certified_mail ==>
+   \<forall>K KK. invKey TTPEncKey \<notin> KK -->
+          (Key K \<in> analz (Key`KK Un (knows Spy evs))) =
+          (K \<in> KK | Key K \<in> analz (knows Spy evs))"
+apply (erule certified_mail.induct)
+apply (drule_tac [6] A=TTP in symKey_neq_priEK) 
+apply (erule_tac [6] disjE [OF hr_form]) 
+apply (drule_tac [5] CM2_S2TTP_analz_knows_Spy) 
+prefer 9
+apply (elim exE)
+apply (simp_all add: synth_analz_insert_eq
+                     subset_trans [OF _ subset_insertI]
+                     subset_trans [OF _ Un_upper2] 
+                del: image_insert image_Un add: analz_image_freshK_simps)
+done
+
+
+lemma analz_insert_freshK:
+  "[| evs \<in> certified_mail;  KAB \<noteq> invKey TTPEncKey |] ==>
+      (Key K \<in> analz (insert (Key KAB) (knows Spy evs))) =
+      (K = KAB | Key K \<in> analz (knows Spy evs))"
+by (simp only: analz_image_freshK analz_image_freshK_simps)
+
+text{*@{term S2TTP} must have originated from a valid sender
+    provided @{term K} is secure.  Proof is surprisingly hard.*}
+
+lemma Notes_SSL_imp_used:
+     "[|Notes B {|Agent A, Agent B, X|} \<in> set evs|] ==> X \<in> used evs"
+by (blast dest!: Notes_imp_used)
+
+
+(*The weaker version, replacing "used evs" by "parts (knows Spy evs)", 
+   isn't inductive: message 3 case can't be proved *)
+lemma S2TTP_sender_lemma [rule_format]:
+ "evs \<in> certified_mail ==>
+    Key K \<notin> analz (knows Spy evs) -->
+    (\<forall>AO. Crypt TTPEncKey
+	   {|Agent S, Number AO, Key K, Agent R, hs|} \<in> used evs -->
+    (\<exists>m ctxt q. 
+        hs = Hash{|Number ctxt, Nonce q, response S R q, Crypt K (Number m)|} &
+	Says S R
+	   {|Agent S, Agent TTP, Crypt K (Number m), Number AO,
+	     Number ctxt, Nonce q,
+	     Crypt TTPEncKey
+	      {|Agent S, Number AO, Key K, Agent R, hs |}|} \<in> set evs))" 
+apply (erule certified_mail.induct, analz_mono_contra)
+apply (drule_tac [5] CM2_S2TTP_parts_knows_Spy, simp)
+apply (simp add: used_Nil Crypt_notin_initState, simp_all)
+txt{*Fake*}
+apply (blast dest: Fake_parts_sing[THEN subsetD]
+             dest!: analz_subset_parts[THEN subsetD])  
+txt{*Fake SSL*}
+apply (blast dest: Fake_parts_sing[THEN subsetD]
+            dest: analz_subset_parts[THEN subsetD])  
+txt{*Message 1*}
+apply clarsimp
+apply blast 
+txt{*Message 2*}
+apply (simp add: parts_insert2, clarify) 
+apply (drule parts_cut, assumption, simp) 
+apply (blast dest: parts_knows_Spy_subset_used [THEN subsetD]) 
+txt{*Message 3*} 
+apply (blast dest: Notes_SSL_imp_used used_parts_subset_parts) 
+done 
+
+lemma S2TTP_sender:
+ "[|Crypt TTPEncKey {|Agent S, Number AO, Key K, Agent R, hs|} \<in> used evs;
+    Key K \<notin> analz (knows Spy evs);
+    evs \<in> certified_mail|]
+  ==> \<exists>m ctxt q. 
+        hs = Hash{|Number ctxt, Nonce q, response S R q, Crypt K (Number m)|} &
+	Says S R
+	   {|Agent S, Agent TTP, Crypt K (Number m), Number AO,
+	     Number ctxt, Nonce q,
+	     Crypt TTPEncKey
+	      {|Agent S, Number AO, Key K, Agent R, hs |}|} \<in> set evs" 
+by (blast intro: S2TTP_sender_lemma) 
+
+
+text{*Nobody can have used non-existent keys!*}
+lemma new_keys_not_used [rule_format, simp]:
+    "[|Key K \<notin> used evs; K \<in> symKeys; evs \<in> certified_mail|]
+     ==> K \<notin> keysFor (parts (spies evs))"
+apply (erule rev_mp) 
+apply (erule certified_mail.induct, simp_all) 
+txt{*Fake*}
+apply (force dest!: keysFor_parts_insert) 
+txt{*Message 1*}
+apply blast 
+txt{*Message 3*}
+apply (frule CM3_k_parts_knows_Spy, assumption)
+apply (frule_tac hr_form, assumption) 
+apply (force dest!: keysFor_parts_insert)
+done
+
+
+text{*Less easy to prove @{term "m'=m"}.  Maybe needs a separate unicity
+theorem fror ciphertexts of the form @{term "Crypt K (Number m)"}, 
+where @{term K} is secure.*}
+lemma Key_unique_lemma [rule_format]:
+     "evs \<in> certified_mail ==>
+       Key K \<notin> analz (knows Spy evs) -->
+       (\<forall>m cleartext q hs.
+        Says S R
+           {|Agent S, Agent TTP, Crypt K (Number m), Number AO,
+             Number cleartext, Nonce q,
+             Crypt TTPEncKey {|Agent S, Number AO, Key K, Agent R, hs|}|}
+          \<in> set evs -->
+       (\<forall>m' cleartext' q' hs'.
+       Says S' R'
+           {|Agent S', Agent TTP, Crypt K (Number m'), Number AO',
+             Number cleartext', Nonce q',
+             Crypt TTPEncKey {|Agent S', Number AO', Key K, Agent R', hs'|}|}
+          \<in> set evs --> R' = R & S' = S & AO' = AO & hs' = hs))" 
+apply (erule certified_mail.induct, analz_mono_contra, simp_all)
+txt{*Fake*} 
+apply (blast dest!: usedI S2TTP_sender analz_subset_parts[THEN subsetD]) 
+txt{*Message 1*}
+apply (blast dest!: Says_imp_knows_Spy [THEN parts.Inj] new_keys_not_used Crypt_imp_keysFor) 
+done
+
+text{*The key determines the sender, recipient and protocol options.*}
+theorem Key_unique:
+      "[|Says S R
+           {|Agent S, Agent TTP, Crypt K (Number m), Number AO,
+             Number cleartext, Nonce q,
+             Crypt TTPEncKey {|Agent S, Number AO, Key K, Agent R, hs|}|}
+          \<in> set evs;
+         Says S' R'
+           {|Agent S', Agent TTP, Crypt K (Number m'), Number AO',
+             Number cleartext', Nonce q',
+             Crypt TTPEncKey {|Agent S', Number AO', Key K, Agent R', hs'|}|}
+          \<in> set evs;
+         Key K \<notin> analz (knows Spy evs);
+         evs \<in> certified_mail|]
+       ==> R' = R & S' = S & AO' = AO & hs' = hs"
+by (rule Key_unique_lemma, assumption+)
+
+text{*If Spy gets the key then @{term R} is bad and also @{term S} at least
+      gets his return receipt (and therefore has no grounds for complaint).*}
+lemma Spy_see_encrypted_key_imp:
+      "[|Says S R {|Agent S, Agent TTP, Crypt K (Number m), Number AO, 
+                     Number cleartext, Nonce q, S2TTP|} \<in> set evs;
+         Key K \<in> analz(knows Spy evs);
+         S2TTP = Crypt TTPEncKey {|Agent S, Number AO, Key K, Agent R, hs|};
+	 evs \<in> certified_mail;
+         S\<noteq>Spy|]
+      ==> R \<in> bad & Says TTP S (Crypt TTPSigKey S2TTP) \<in> set evs"
+apply (erule rev_mp)
+apply (erule rev_mp)
+apply (erule ssubst)
+apply (erule certified_mail.induct, simp_all)
+txt{*Fake*}
+apply spy_analz
+txt{*Fake SSL*}
+apply spy_analz
+txt{*Message 3*}
+apply (frule_tac hr_form, assumption)
+apply (elim disjE exE) 
+apply (simp_all add: synth_analz_insert_eq  
+                     subset_trans [OF _ subset_insertI]
+                     subset_trans [OF _ Un_upper2] 
+                del: image_insert image_Un add: analz_image_freshK_simps) 
+apply (simp_all add: symKey_neq_priEK analz_insert_freshK)
+apply (blast dest: Notes_SSL_imp_used S2TTP_sender Key_unique)+
+done
+
+text{*Confidentially for the symmetric key*}
+theorem Spy_not_see_encrypted_key:
+      "[|Says S R {|Agent S, Agent TTP, Crypt K (Number m), Number AO, 
+                     Number cleartext, Nonce q, S2TTP|} \<in> set evs;
+         S2TTP = Crypt TTPEncKey {|Agent S, Number AO, Key K, Agent R, hs|};
+	 evs \<in> certified_mail;
+         S\<noteq>Spy; R \<notin> bad|]
+      ==> Key K \<notin> analz(knows Spy evs)"
+by (blast dest: Spy_see_encrypted_key_imp) 
+
+
+subsection{*The Guarantees for Sender and Recipient*}
+
+text{*Agent @{term R}, who may be the Spy, doesn't receive the key
+ until @{term S} has access to the return receipt.*} 
+theorem S_guarantee:
+      "[|Notes R {|Agent TTP, Agent R, Key K, hs|} \<in> set evs;
+         Says S R {|Agent S, Agent TTP, Crypt K (Number m), Number AO, 
+                     Number cleartext, Nonce q, S2TTP|} \<in> set evs;
+         S2TTP = Crypt TTPEncKey {|Agent S, Number AO, Key K, Agent R, hs|};
+         hs = Hash {|Number cleartext, Nonce q, response S R q, 
+                     Crypt K (Number m)|};
+         S\<noteq>Spy;  evs \<in> certified_mail|]
+      ==> Says TTP S (Crypt TTPSigKey S2TTP) \<in> set evs"
+apply (erule rev_mp)
+apply (erule rev_mp)
+apply (erule ssubst)
+apply (erule ssubst)
+apply (erule certified_mail.induct, simp_all)
+txt{*Message 1*}
+apply (blast dest: Notes_imp_used) 
+txt{*Message 3*} 
+apply (blast dest: Notes_SSL_imp_used S2TTP_sender Key_unique 
+                   Spy_see_encrypted_key_imp) 
+done
+
+
+lemma Says_TTP_imp_Notes:
+  "[|Says TTP S (Crypt TTPSigKey S2TTP) \<in> set evs;
+     S2TTP = Crypt TTPEncKey {|Agent S, Number AO, Key K, Agent R,
+	         Hash {|Number cleartext, Nonce q, r, em|}|};
+     evs \<in> certified_mail|]
+   ==> Notes TTP
+	   {|Agent R, Agent TTP, S2TTP, Key (RPwd R),
+	     Hash {|Number cleartext, Nonce q, r, em|}|}
+	  \<in> set evs"
+apply (erule rev_mp)
+apply (erule ssubst) 
+apply (erule certified_mail.induct, simp_all)
+done
+
+
+
+text{*Recipient's guarantee: if @{term R} sends message 2, and
+     @{term S} gets a delivery certificate, then @{term R}
+     receives the necessary key.*}
+theorem R_guarantee:
+  "[|Notes TTP {|Agent R, Agent TTP, S2TTP, Key(RPwd R), hr|} \<in> set evs;
+     Says TTP S (Crypt TTPSigKey S2TTP) \<in> set evs;
+     S2TTP = Crypt TTPEncKey {|Agent S, Number AO, Key K, Agent R,
+	         Hash {|Number cleartext, Nonce q, r, em|}|};
+     hr = Hash {|Number cleartext, Nonce q, r, em|};
+     R\<noteq>Spy;  evs \<in> certified_mail|]
+  ==> Notes R {|Agent TTP, Agent R, Key K, hr|} \<in> set evs"
+apply (erule rev_mp)
+apply (erule rev_mp)
+apply (erule ssubst)
+apply (erule ssubst)
+apply (erule certified_mail.induct, simp_all)
+txt{*Message 2*}
+apply clarify
+apply (drule Says_TTP_imp_Notes [OF _ refl], assumption)
+apply simp  
+done
+
+end
