src/HOL/Auth/NS_Public.thy
@@ -24,21 +24,21 @@ inductive ns_public
 
          (*Alice initiates a protocol run, sending a nonce to Bob*)
    NS1:  "\<lbrakk>evs1 \<in> ns_public;  Nonce NA \<notin> used evs1\<rbrakk>
-          \<Longrightarrow> Says A B (Crypt (pubK B) \<lbrace>Nonce NA, Agent A\<rbrace>)
+          \<Longrightarrow> Says A B (Crypt (pubEK B) \<lbrace>Nonce NA, Agent A\<rbrace>)
                  # evs1  \<in>  ns_public"
 
          (*Bob responds to Alice's message with a further nonce*)
    NS2:  "\<lbrakk>evs2 \<in> ns_public;  Nonce NB \<notin> used evs2;
-           Says A' B (Crypt (pubK B) \<lbrace>Nonce NA, Agent A\<rbrace>) \<in> set evs2\<rbrakk>
-          \<Longrightarrow> Says B A (Crypt (pubK A) \<lbrace>Nonce NA, Nonce NB, Agent B\<rbrace>)
+           Says A' B (Crypt (pubEK B) \<lbrace>Nonce NA, Agent A\<rbrace>) \<in> set evs2\<rbrakk>
+          \<Longrightarrow> Says B A (Crypt (pubEK A) \<lbrace>Nonce NA, Nonce NB, Agent B\<rbrace>)
                 # evs2  \<in>  ns_public"
 
          (*Alice proves her existence by sending NB back to Bob.*)
    NS3:  "\<lbrakk>evs3 \<in> ns_public;
-           Says A  B (Crypt (pubK B) \<lbrace>Nonce NA, Agent A\<rbrace>) \<in> set evs3;
-           Says B' A (Crypt (pubK A) \<lbrace>Nonce NA, Nonce NB, Agent B\<rbrace>)
+           Says A  B (Crypt (pubEK B) \<lbrace>Nonce NA, Agent A\<rbrace>) \<in> set evs3;
+           Says B' A (Crypt (pubEK A) \<lbrace>Nonce NA, Nonce NB, Agent B\<rbrace>)
               \<in> set evs3\<rbrakk>
-          \<Longrightarrow> Says A B (Crypt (pubK B) (Nonce NB)) # evs3 \<in> ns_public"
+          \<Longrightarrow> Says A B (Crypt (pubEK B) (Nonce NB)) # evs3 \<in> ns_public"
 
 declare knows_Spy_partsEs [elim]
 declare analz_subset_parts [THEN subsetD, dest]
@@ -46,7 +46,7 @@ declare Fake_parts_insert [THEN subsetD, dest]
 declare image_eq_UN [simp]  (*accelerates proofs involving nested images*)
 
 (*A "possibility property": there are traces that reach the end*)
-lemma "\<exists>NB. \<exists>evs \<in> ns_public. Says A B (Crypt (pubK B) (Nonce NB)) \<in> set evs"
+lemma "\<exists>NB. \<exists>evs \<in> ns_public. Says A B (Crypt (pubEK B) (Nonce NB)) \<in> set evs"
 apply (intro exI bexI)
 apply (rule_tac [2] ns_public.Nil [THEN ns_public.NS1, THEN ns_public.NS2, 
                                    THEN ns_public.NS3])
@@ -59,12 +59,12 @@ by possibility
     sends messages containing X! **)
 
 (*Spy never sees another agent's private key! (unless it's bad at start)*)
-lemma Spy_see_priK [simp]: 
-      "evs \<in> ns_public \<Longrightarrow> (Key (priK A) \<in> parts (spies evs)) = (A \<in> bad)"
+lemma Spy_see_priEK [simp]: 
+      "evs \<in> ns_public \<Longrightarrow> (Key (priEK A) \<in> parts (spies evs)) = (A \<in> bad)"
 by (erule ns_public.induct, auto)
 
-lemma Spy_analz_priK [simp]: 
-      "evs \<in> ns_public \<Longrightarrow> (Key (priK A) \<in> analz (spies evs)) = (A \<in> bad)"
+lemma Spy_analz_priEK [simp]: 
+      "evs \<in> ns_public \<Longrightarrow> (Key (priEK A) \<in> analz (spies evs)) = (A \<in> bad)"
 by auto
 
 
@@ -75,8 +75,8 @@ by auto
   is secret.  (Honest users generate fresh nonces.)*)
 lemma no_nonce_NS1_NS2 [rule_format]: 
       "evs \<in> ns_public 
-       \<Longrightarrow> Crypt (pubK C) \<lbrace>NA', Nonce NA, Agent D\<rbrace> \<in> parts (spies evs) \<longrightarrow>
-           Crypt (pubK B) \<lbrace>Nonce NA, Agent A\<rbrace> \<in> parts (spies evs) \<longrightarrow>  
+       \<Longrightarrow> Crypt (pubEK C) \<lbrace>NA', Nonce NA, Agent D\<rbrace> \<in> parts (spies evs) \<longrightarrow>
+           Crypt (pubEK B) \<lbrace>Nonce NA, Agent A\<rbrace> \<in> parts (spies evs) \<longrightarrow>  
            Nonce NA \<in> analz (spies evs)"
 apply (erule ns_public.induct, simp_all)
 apply (blast intro: analz_insertI)+
@@ -84,8 +84,8 @@ done
 
 (*Unicity for NS1: nonce NA identifies agents A and B*)
 lemma unique_NA: 
-     "\<lbrakk>Crypt(pubK B)  \<lbrace>Nonce NA, Agent A \<rbrace> \<in> parts(spies evs);  
-       Crypt(pubK B') \<lbrace>Nonce NA, Agent A'\<rbrace> \<in> parts(spies evs);  
+     "\<lbrakk>Crypt(pubEK B)  \<lbrace>Nonce NA, Agent A \<rbrace> \<in> parts(spies evs);  
+       Crypt(pubEK B') \<lbrace>Nonce NA, Agent A'\<rbrace> \<in> parts(spies evs);  
        Nonce NA \<notin> analz (spies evs); evs \<in> ns_public\<rbrakk>
       \<Longrightarrow> A=A' \<and> B=B'"
 apply (erule rev_mp, erule rev_mp, erule rev_mp)   
@@ -99,7 +99,7 @@ done
   The major premise "Says A B ..." makes it a dest-rule, so we use
   (erule rev_mp) rather than rule_format. *)
 theorem Spy_not_see_NA: 
-      "\<lbrakk>Says A B (Crypt(pubK B) \<lbrace>Nonce NA, Agent A\<rbrace>) \<in> set evs;
+      "\<lbrakk>Says A B (Crypt(pubEK B) \<lbrace>Nonce NA, Agent A\<rbrace>) \<in> set evs;
         A \<notin> bad;  B \<notin> bad;  evs \<in> ns_public\<rbrakk>                     
        \<Longrightarrow> Nonce NA \<notin> analz (spies evs)"
 apply (erule rev_mp)   
@@ -112,28 +112,28 @@ done
   to start a run, then B has sent message 2.*)
 lemma A_trusts_NS2_lemma [rule_format]: 
    "\<lbrakk>A \<notin> bad;  B \<notin> bad;  evs \<in> ns_public\<rbrakk>                     
-    \<Longrightarrow> Crypt (pubK A) \<lbrace>Nonce NA, Nonce NB, Agent B\<rbrace> \<in> parts (spies evs) \<longrightarrow>
-	Says A B (Crypt(pubK B) \<lbrace>Nonce NA, Agent A\<rbrace>) \<in> set evs \<longrightarrow>
-	Says B A (Crypt(pubK A) \<lbrace>Nonce NA, Nonce NB, Agent B\<rbrace>) \<in> set evs"
+    \<Longrightarrow> Crypt (pubEK A) \<lbrace>Nonce NA, Nonce NB, Agent B\<rbrace> \<in> parts (spies evs) \<longrightarrow>
+	Says A B (Crypt(pubEK B) \<lbrace>Nonce NA, Agent A\<rbrace>) \<in> set evs \<longrightarrow>
+	Says B A (Crypt(pubEK A) \<lbrace>Nonce NA, Nonce NB, Agent B\<rbrace>) \<in> set evs"
 apply (erule ns_public.induct, simp_all)
 (*Fake, NS1*)
 apply (blast dest: Spy_not_see_NA)+
 done
 
 theorem A_trusts_NS2: 
-     "\<lbrakk>Says A  B (Crypt(pubK B) \<lbrace>Nonce NA, Agent A\<rbrace>) \<in> set evs;   
-       Says B' A (Crypt(pubK A) \<lbrace>Nonce NA, Nonce NB, Agent B\<rbrace>) \<in> set evs;
+     "\<lbrakk>Says A  B (Crypt(pubEK B) \<lbrace>Nonce NA, Agent A\<rbrace>) \<in> set evs;   
+       Says B' A (Crypt(pubEK A) \<lbrace>Nonce NA, Nonce NB, Agent B\<rbrace>) \<in> set evs;
        A \<notin> bad;  B \<notin> bad;  evs \<in> ns_public\<rbrakk>                     
-      \<Longrightarrow> Says B A (Crypt(pubK A) \<lbrace>Nonce NA, Nonce NB, Agent B\<rbrace>) \<in> set evs"
+      \<Longrightarrow> Says B A (Crypt(pubEK A) \<lbrace>Nonce NA, Nonce NB, Agent B\<rbrace>) \<in> set evs"
 by (blast intro: A_trusts_NS2_lemma)
 
 
 (*If the encrypted message appears then it originated with Alice in NS1*)
 lemma B_trusts_NS1 [rule_format]:
      "evs \<in> ns_public                                         
-      \<Longrightarrow> Crypt (pubK B) \<lbrace>Nonce NA, Agent A\<rbrace> \<in> parts (spies evs) \<longrightarrow>
+      \<Longrightarrow> Crypt (pubEK B) \<lbrace>Nonce NA, Agent A\<rbrace> \<in> parts (spies evs) \<longrightarrow>
 	  Nonce NA \<notin> analz (spies evs) \<longrightarrow>
-	  Says A B (Crypt (pubK B) \<lbrace>Nonce NA, Agent A\<rbrace>) \<in> set evs"
+	  Says A B (Crypt (pubEK B) \<lbrace>Nonce NA, Agent A\<rbrace>) \<in> set evs"
 apply (erule ns_public.induct, simp_all)
 (*Fake*)
 apply (blast intro!: analz_insertI)
@@ -148,8 +148,8 @@ done
   [proof closely follows that for unique_NA] *)
 
 lemma unique_NB [dest]: 
-     "\<lbrakk>Crypt(pubK A)  \<lbrace>Nonce NA, Nonce NB, Agent B\<rbrace> \<in> parts(spies evs);
-       Crypt(pubK A') \<lbrace>Nonce NA', Nonce NB, Agent B'\<rbrace> \<in> parts(spies evs);
+     "\<lbrakk>Crypt(pubEK A)  \<lbrace>Nonce NA, Nonce NB, Agent B\<rbrace> \<in> parts(spies evs);
+       Crypt(pubEK A') \<lbrace>Nonce NA', Nonce NB, Agent B'\<rbrace> \<in> parts(spies evs);
        Nonce NB \<notin> analz (spies evs); evs \<in> ns_public\<rbrakk>
       \<Longrightarrow> A=A' \<and> NA=NA' \<and> B=B'"
 apply (erule rev_mp, erule rev_mp, erule rev_mp)   
@@ -161,7 +161,7 @@ done
 
 (*Secrecy: Spy does not see the nonce sent in msg NS2 if A and B are secure*)
 theorem Spy_not_see_NB [dest]:
-     "\<lbrakk>Says B A (Crypt (pubK A) \<lbrace>Nonce NA, Nonce NB, Agent B\<rbrace>) \<in> set evs;
+     "\<lbrakk>Says B A (Crypt (pubEK A) \<lbrace>Nonce NA, Nonce NB, Agent B\<rbrace>) \<in> set evs;
        A \<notin> bad;  B \<notin> bad;  evs \<in> ns_public\<rbrakk>
       \<Longrightarrow> Nonce NB \<notin> analz (spies evs)"
 apply (erule rev_mp)
@@ -174,16 +174,16 @@ done
   in message 2, then A has sent message 3.*)
 lemma B_trusts_NS3_lemma [rule_format]:
      "\<lbrakk>A \<notin> bad;  B \<notin> bad;  evs \<in> ns_public\<rbrakk> \<Longrightarrow>
-      Crypt (pubK B) (Nonce NB) \<in> parts (spies evs) \<longrightarrow>
-      Says B A (Crypt (pubK A) \<lbrace>Nonce NA, Nonce NB, Agent B\<rbrace>) \<in> set evs \<longrightarrow>
-      Says A B (Crypt (pubK B) (Nonce NB)) \<in> set evs"
+      Crypt (pubEK B) (Nonce NB) \<in> parts (spies evs) \<longrightarrow>
+      Says B A (Crypt (pubEK A) \<lbrace>Nonce NA, Nonce NB, Agent B\<rbrace>) \<in> set evs \<longrightarrow>
+      Says A B (Crypt (pubEK B) (Nonce NB)) \<in> set evs"
 by (erule ns_public.induct, auto)
 
 theorem B_trusts_NS3:
-     "\<lbrakk>Says B A  (Crypt (pubK A) \<lbrace>Nonce NA, Nonce NB, Agent B\<rbrace>) \<in> set evs;
-       Says A' B (Crypt (pubK B) (Nonce NB)) \<in> set evs;             
+     "\<lbrakk>Says B A  (Crypt (pubEK A) \<lbrace>Nonce NA, Nonce NB, Agent B\<rbrace>) \<in> set evs;
+       Says A' B (Crypt (pubEK B) (Nonce NB)) \<in> set evs;             
        A \<notin> bad;  B \<notin> bad;  evs \<in> ns_public\<rbrakk>                    
-      \<Longrightarrow> Says A B (Crypt (pubK B) (Nonce NB)) \<in> set evs"
+      \<Longrightarrow> Says A B (Crypt (pubEK B) (Nonce NB)) \<in> set evs"
 by (blast intro: B_trusts_NS3_lemma)
 
 (*** Overall guarantee for B ***)
@@ -193,9 +193,9 @@ by (blast intro: B_trusts_NS3_lemma)
   NA, then A initiated the run using NA.*)
 theorem B_trusts_protocol:
      "\<lbrakk>A \<notin> bad;  B \<notin> bad;  evs \<in> ns_public\<rbrakk> \<Longrightarrow>
-      Crypt (pubK B) (Nonce NB) \<in> parts (spies evs) \<longrightarrow>
-      Says B A  (Crypt (pubK A) \<lbrace>Nonce NA, Nonce NB, Agent B\<rbrace>) \<in> set evs \<longrightarrow>
-      Says A B (Crypt (pubK B) \<lbrace>Nonce NA, Agent A\<rbrace>) \<in> set evs"
+      Crypt (pubEK B) (Nonce NB) \<in> parts (spies evs) \<longrightarrow>
+      Says B A  (Crypt (pubEK A) \<lbrace>Nonce NA, Nonce NB, Agent B\<rbrace>) \<in> set evs \<longrightarrow>
+      Says A B (Crypt (pubEK B) \<lbrace>Nonce NA, Agent A\<rbrace>) \<in> set evs"
 by (erule ns_public.induct, auto)
 
 end
