src/HOL/Auth/NS_Public_Bad.thy
@@ -28,20 +28,20 @@ inductive ns_public
 
          (*Alice initiates a protocol run, sending a nonce to Bob*)
    NS1:  "\<lbrakk>evs1 \<in> ns_public;  Nonce NA \<notin> used evs1\<rbrakk>
-          \<Longrightarrow> Says A B (Crypt (pubK B) \<lbrace>Nonce NA, Agent A\<rbrace>)
+          \<Longrightarrow> Says A B (Crypt (pubEK B) \<lbrace>Nonce NA, Agent A\<rbrace>)
                 # evs1  \<in>  ns_public"
 
          (*Bob responds to Alice's message with a further nonce*)
    NS2:  "\<lbrakk>evs2 \<in> ns_public;  Nonce NB \<notin> used evs2;
-           Says A' B (Crypt (pubK B) \<lbrace>Nonce NA, Agent A\<rbrace>) \<in> set evs2\<rbrakk>
-          \<Longrightarrow> Says B A (Crypt (pubK A) \<lbrace>Nonce NA, Nonce NB\<rbrace>)
+           Says A' B (Crypt (pubEK B) \<lbrace>Nonce NA, Agent A\<rbrace>) \<in> set evs2\<rbrakk>
+          \<Longrightarrow> Says B A (Crypt (pubEK A) \<lbrace>Nonce NA, Nonce NB\<rbrace>)
                 # evs2  \<in>  ns_public"
 
          (*Alice proves her existence by sending NB back to Bob.*)
    NS3:  "\<lbrakk>evs3 \<in> ns_public;
-           Says A  B (Crypt (pubK B) \<lbrace>Nonce NA, Agent A\<rbrace>) \<in> set evs3;
-           Says B' A (Crypt (pubK A) \<lbrace>Nonce NA, Nonce NB\<rbrace>) \<in> set evs3\<rbrakk>
-          \<Longrightarrow> Says A B (Crypt (pubK B) (Nonce NB)) # evs3 \<in> ns_public"
+           Says A  B (Crypt (pubEK B) \<lbrace>Nonce NA, Agent A\<rbrace>) \<in> set evs3;
+           Says B' A (Crypt (pubEK A) \<lbrace>Nonce NA, Nonce NB\<rbrace>) \<in> set evs3\<rbrakk>
+          \<Longrightarrow> Says A B (Crypt (pubEK B) (Nonce NB)) # evs3 \<in> ns_public"
 
 declare knows_Spy_partsEs [elim]
 declare analz_subset_parts [THEN subsetD, dest]
@@ -49,7 +49,7 @@ declare Fake_parts_insert [THEN subsetD, dest]
 declare image_eq_UN [simp]  (*accelerates proofs involving nested images*)
 
 (*A "possibility property": there are traces that reach the end*)
-lemma "\<exists>NB. \<exists>evs \<in> ns_public. Says A B (Crypt (pubK B) (Nonce NB)) \<in> set evs"
+lemma "\<exists>NB. \<exists>evs \<in> ns_public. Says A B (Crypt (pubEK B) (Nonce NB)) \<in> set evs"
 apply (intro exI bexI)
 apply (rule_tac [2] ns_public.Nil [THEN ns_public.NS1, THEN ns_public.NS2, 
                                    THEN ns_public.NS3])
@@ -62,12 +62,12 @@ by possibility
     sends messages containing X! **)
 
 (*Spy never sees another agent's private key! (unless it's bad at start)*)
-lemma Spy_see_priK [simp]: 
-      "evs \<in> ns_public \<Longrightarrow> (Key (priK A) \<in> parts (spies evs)) = (A \<in> bad)"
+lemma Spy_see_priEK [simp]: 
+      "evs \<in> ns_public \<Longrightarrow> (Key (priEK A) \<in> parts (spies evs)) = (A \<in> bad)"
 by (erule ns_public.induct, auto)
 
-lemma Spy_analz_priK [simp]: 
-      "evs \<in> ns_public \<Longrightarrow> (Key (priK A) \<in> analz (spies evs)) = (A \<in> bad)"
+lemma Spy_analz_priEK [simp]: 
+      "evs \<in> ns_public \<Longrightarrow> (Key (priEK A) \<in> analz (spies evs)) = (A \<in> bad)"
 by auto
 
 
@@ -77,8 +77,8 @@ by auto
   is secret.  (Honest users generate fresh nonces.)*)
 lemma no_nonce_NS1_NS2 [rule_format]: 
       "evs \<in> ns_public 
-       \<Longrightarrow> Crypt (pubK C) \<lbrace>NA', Nonce NA\<rbrace> \<in> parts (spies evs) \<longrightarrow>
-           Crypt (pubK B) \<lbrace>Nonce NA, Agent A\<rbrace> \<in> parts (spies evs) \<longrightarrow>  
+       \<Longrightarrow> Crypt (pubEK C) \<lbrace>NA', Nonce NA\<rbrace> \<in> parts (spies evs) \<longrightarrow>
+           Crypt (pubEK B) \<lbrace>Nonce NA, Agent A\<rbrace> \<in> parts (spies evs) \<longrightarrow>  
            Nonce NA \<in> analz (spies evs)"
 apply (erule ns_public.induct, simp_all)
 apply (blast intro: analz_insertI)+
@@ -87,8 +87,8 @@ done
 
 (*Unicity for NS1: nonce NA identifies agents A and B*)
 lemma unique_NA: 
-     "\<lbrakk>Crypt(pubK B)  \<lbrace>Nonce NA, Agent A \<rbrace> \<in> parts(spies evs);  
-       Crypt(pubK B') \<lbrace>Nonce NA, Agent A'\<rbrace> \<in> parts(spies evs);  
+     "\<lbrakk>Crypt(pubEK B)  \<lbrace>Nonce NA, Agent A \<rbrace> \<in> parts(spies evs);  
+       Crypt(pubEK B') \<lbrace>Nonce NA, Agent A'\<rbrace> \<in> parts(spies evs);  
        Nonce NA \<notin> analz (spies evs); evs \<in> ns_public\<rbrakk>
       \<Longrightarrow> A=A' \<and> B=B'"
 apply (erule rev_mp, erule rev_mp, erule rev_mp)   
@@ -102,7 +102,7 @@ done
   The major premise "Says A B ..." makes it a dest-rule, so we use
   (erule rev_mp) rather than rule_format. *)
 theorem Spy_not_see_NA: 
-      "\<lbrakk>Says A B (Crypt(pubK B) \<lbrace>Nonce NA, Agent A\<rbrace>) \<in> set evs;
+      "\<lbrakk>Says A B (Crypt(pubEK B) \<lbrace>Nonce NA, Agent A\<rbrace>) \<in> set evs;
         A \<notin> bad;  B \<notin> bad;  evs \<in> ns_public\<rbrakk>                     
        \<Longrightarrow> Nonce NA \<notin> analz (spies evs)"
 apply (erule rev_mp)   
@@ -115,27 +115,27 @@ done
   to start a run, then B has sent message 2.*)
 lemma A_trusts_NS2_lemma [rule_format]: 
    "\<lbrakk>A \<notin> bad;  B \<notin> bad;  evs \<in> ns_public\<rbrakk>                     
-    \<Longrightarrow> Crypt (pubK A) \<lbrace>Nonce NA, Nonce NB\<rbrace> \<in> parts (spies evs) \<longrightarrow>
-	Says A B (Crypt(pubK B) \<lbrace>Nonce NA, Agent A\<rbrace>) \<in> set evs \<longrightarrow>
-	Says B A (Crypt(pubK A) \<lbrace>Nonce NA, Nonce NB\<rbrace>) \<in> set evs"
+    \<Longrightarrow> Crypt (pubEK A) \<lbrace>Nonce NA, Nonce NB\<rbrace> \<in> parts (spies evs) \<longrightarrow>
+	Says A B (Crypt(pubEK B) \<lbrace>Nonce NA, Agent A\<rbrace>) \<in> set evs \<longrightarrow>
+	Says B A (Crypt(pubEK A) \<lbrace>Nonce NA, Nonce NB\<rbrace>) \<in> set evs"
 apply (erule ns_public.induct)
 apply (auto dest: Spy_not_see_NA unique_NA)
 done
 
 theorem A_trusts_NS2: 
-     "\<lbrakk>Says A  B (Crypt(pubK B) \<lbrace>Nonce NA, Agent A\<rbrace>) \<in> set evs;   
-       Says B' A (Crypt(pubK A) \<lbrace>Nonce NA, Nonce NB\<rbrace>) \<in> set evs;
+     "\<lbrakk>Says A  B (Crypt(pubEK B) \<lbrace>Nonce NA, Agent A\<rbrace>) \<in> set evs;   
+       Says B' A (Crypt(pubEK A) \<lbrace>Nonce NA, Nonce NB\<rbrace>) \<in> set evs;
        A \<notin> bad;  B \<notin> bad;  evs \<in> ns_public\<rbrakk>                     
-      \<Longrightarrow> Says B A (Crypt(pubK A) \<lbrace>Nonce NA, Nonce NB\<rbrace>) \<in> set evs"
+      \<Longrightarrow> Says B A (Crypt(pubEK A) \<lbrace>Nonce NA, Nonce NB\<rbrace>) \<in> set evs"
 by (blast intro: A_trusts_NS2_lemma)
 
 
 (*If the encrypted message appears then it originated with Alice in NS1*)
 lemma B_trusts_NS1 [rule_format]:
      "evs \<in> ns_public                                         
-      \<Longrightarrow> Crypt (pubK B) \<lbrace>Nonce NA, Agent A\<rbrace> \<in> parts (spies evs) \<longrightarrow>
+      \<Longrightarrow> Crypt (pubEK B) \<lbrace>Nonce NA, Agent A\<rbrace> \<in> parts (spies evs) \<longrightarrow>
 	  Nonce NA \<notin> analz (spies evs) \<longrightarrow>
-	  Says A B (Crypt (pubK B) \<lbrace>Nonce NA, Agent A\<rbrace>) \<in> set evs"
+	  Says A B (Crypt (pubEK B) \<lbrace>Nonce NA, Agent A\<rbrace>) \<in> set evs"
 apply (erule ns_public.induct, simp_all)
 (*Fake*)
 apply (blast intro!: analz_insertI)
@@ -148,8 +148,8 @@ done
 (*Unicity for NS2: nonce NB identifies nonce NA and agent A
   [proof closely follows that for unique_NA] *)
 lemma unique_NB [dest]: 
-     "\<lbrakk>Crypt(pubK A)  \<lbrace>Nonce NA, Nonce NB\<rbrace> \<in> parts(spies evs);
-       Crypt(pubK A') \<lbrace>Nonce NA', Nonce NB\<rbrace> \<in> parts(spies evs);
+     "\<lbrakk>Crypt(pubEK A)  \<lbrace>Nonce NA, Nonce NB\<rbrace> \<in> parts(spies evs);
+       Crypt(pubEK A') \<lbrace>Nonce NA', Nonce NB\<rbrace> \<in> parts(spies evs);
        Nonce NB \<notin> analz (spies evs); evs \<in> ns_public\<rbrakk>
      \<Longrightarrow> A=A' \<and> NA=NA'"
 apply (erule rev_mp, erule rev_mp, erule rev_mp)   
@@ -161,8 +161,8 @@ done
 
 (*NB remains secret PROVIDED Alice never responds with round 3*)
 theorem Spy_not_see_NB [dest]:
-     "\<lbrakk>Says B A (Crypt (pubK A) \<lbrace>Nonce NA, Nonce NB\<rbrace>) \<in> set evs;   
-       \<forall>C. Says A C (Crypt (pubK C) (Nonce NB)) \<notin> set evs;       
+     "\<lbrakk>Says B A (Crypt (pubEK A) \<lbrace>Nonce NA, Nonce NB\<rbrace>) \<in> set evs;   
+       \<forall>C. Says A C (Crypt (pubEK C) (Nonce NB)) \<notin> set evs;       
        A \<notin> bad;  B \<notin> bad;  evs \<in> ns_public\<rbrakk>                      
      \<Longrightarrow> Nonce NB \<notin> analz (spies evs)"
 apply (erule rev_mp, erule rev_mp)
@@ -177,23 +177,23 @@ done
 
 lemma B_trusts_NS3_lemma [rule_format]:
      "\<lbrakk>A \<notin> bad;  B \<notin> bad;  evs \<in> ns_public\<rbrakk>                    
-      \<Longrightarrow> Crypt (pubK B) (Nonce NB) \<in> parts (spies evs) \<longrightarrow>
-          Says B A  (Crypt (pubK A) \<lbrace>Nonce NA, Nonce NB\<rbrace>) \<in> set evs \<longrightarrow>
-          (\<exists>C. Says A C (Crypt (pubK C) (Nonce NB)) \<in> set evs)"
+      \<Longrightarrow> Crypt (pubEK B) (Nonce NB) \<in> parts (spies evs) \<longrightarrow>
+          Says B A  (Crypt (pubEK A) \<lbrace>Nonce NA, Nonce NB\<rbrace>) \<in> set evs \<longrightarrow>
+          (\<exists>C. Says A C (Crypt (pubEK C) (Nonce NB)) \<in> set evs)"
 apply (erule ns_public.induct, auto)
 by (blast intro: no_nonce_NS1_NS2)+
 
 theorem B_trusts_NS3:
-     "\<lbrakk>Says B A  (Crypt (pubK A) \<lbrace>Nonce NA, Nonce NB\<rbrace>) \<in> set evs;
-       Says A' B (Crypt (pubK B) (Nonce NB)) \<in> set evs;             
+     "\<lbrakk>Says B A  (Crypt (pubEK A) \<lbrace>Nonce NA, Nonce NB\<rbrace>) \<in> set evs;
+       Says A' B (Crypt (pubEK B) (Nonce NB)) \<in> set evs;             
        A \<notin> bad;  B \<notin> bad;  evs \<in> ns_public\<rbrakk>                    
-      \<Longrightarrow> \<exists>C. Says A C (Crypt (pubK C) (Nonce NB)) \<in> set evs"
+      \<Longrightarrow> \<exists>C. Says A C (Crypt (pubEK C) (Nonce NB)) \<in> set evs"
 by (blast intro: B_trusts_NS3_lemma)
 
 
 (*Can we strengthen the secrecy theorem Spy_not_see_NB?  NO*)
 lemma "\<lbrakk>A \<notin> bad;  B \<notin> bad;  evs \<in> ns_public\<rbrakk>            
-       \<Longrightarrow> Says B A (Crypt (pubK A) \<lbrace>Nonce NA, Nonce NB\<rbrace>) \<in> set evs  
+       \<Longrightarrow> Says B A (Crypt (pubEK A) \<lbrace>Nonce NA, Nonce NB\<rbrace>) \<in> set evs  
            \<longrightarrow> Nonce NB \<notin> analz (spies evs)"
 apply (erule ns_public.induct, simp_all, spy_analz)
 (*NS1: by freshness*)
@@ -211,14 +211,14 @@ oops
 THIS IS THE ATTACK!
 Level 8
 !!evs. \<lbrakk>A \<notin> bad; B \<notin> bad; evs \<in> ns_public\<rbrakk>
-       \<Longrightarrow> Says B A (Crypt (pubK A) \<lbrace>Nonce NA, Nonce NB\<rbrace>) \<in> set evs \<longrightarrow>
+       \<Longrightarrow> Says B A (Crypt (pubEK A) \<lbrace>Nonce NA, Nonce NB\<rbrace>) \<in> set evs \<longrightarrow>
            Nonce NB \<notin> analz (spies evs)
  1. !!C B' evs3.
        \<lbrakk>A \<notin> bad; B \<notin> bad; evs3 \<in> ns_public
-        Says A C (Crypt (pubK C) \<lbrace>Nonce NA, Agent A\<rbrace>) \<in> set evs3;
-        Says B' A (Crypt (pubK A) \<lbrace>Nonce NA, Nonce NB\<rbrace>) \<in> set evs3; 
+        Says A C (Crypt (pubEK C) \<lbrace>Nonce NA, Agent A\<rbrace>) \<in> set evs3;
+        Says B' A (Crypt (pubEK A) \<lbrace>Nonce NA, Nonce NB\<rbrace>) \<in> set evs3; 
         C \<in> bad;
-        Says B A (Crypt (pubK A) \<lbrace>Nonce NA, Nonce NB\<rbrace>) \<in> set evs3;
+        Says B A (Crypt (pubEK A) \<lbrace>Nonce NA, Nonce NB\<rbrace>) \<in> set evs3;
         Nonce NB \<notin> analz (spies evs3)\<rbrakk>
        \<Longrightarrow> False
 *)
