src/HOL/Auth/Public.thy
@@ -8,44 +8,431 @@ Theory of Public Keys (common to all public-key protocols)
 Private and public keys; initial states of agents
 *)
 
-theory Public = Event
-files ("Public_lemmas.ML"):
+theory Public = Event:
+
+subsection{*Asymmetric Keys*}
 
 consts
-  pubK    :: "agent => key"
+  (*the bool is TRUE if a signing key*)
+  publicKey :: "[bool,agent] => key"
 
 syntax
-  priK    :: "agent => key"
+  pubEK :: "agent => key"
+  pubSK :: "agent => key"
 
-translations  (*BEWARE! expressions like  (inj priK)  will NOT work!*)
-  "priK x"  == "invKey(pubK x)"
+  privateKey :: "[bool,agent] => key"
+  priEK :: "agent => key"
+  priSK :: "agent => key"
 
-primrec
-        (*Agents know their private key and all public keys*)
-  initState_Server:  "initState Server     =    
- 		         insert (Key (priK Server)) (Key ` range pubK)"
-  initState_Friend:  "initState (Friend i) =    
- 		         insert (Key (priK (Friend i))) (Key ` range pubK)"
-  initState_Spy:     "initState Spy        =    
- 		         (Key`invKey`pubK`bad) Un (Key ` range pubK)"
+translations
+  "pubEK"  == "publicKey False"
+  "pubSK"  == "publicKey True"
+
+  (*BEWARE!! priEK, priSK DON'T WORK with inj, range, image, etc.*)
+  "privateKey b A" == "invKey (publicKey b A)"
+  "priEK A"  == "privateKey False A"
+  "priSK A"  == "privateKey True A"
+
+
+text{*These translations give backward compatibility.  They represent the
+simple situation where the signature and encryption keys are the same.*}
+syntax
+  pubK :: "agent => key"
+  priK :: "agent => key"
+
+translations
+  "pubK A" == "pubEK A"
+  "priK A" == "invKey (pubEK A)"
 
 
 axioms
-  (*Public keys are disjoint, and never clash with private keys*)
-  inj_pubK:        "inj pubK"
-  priK_neq_pubK:   "priK A ~= pubK B"
+  (*By freeness of agents, no two agents have the same key.  Since true\<noteq>false,
+    no agent has identical signing and encryption keys*)
+  injective_publicKey:
+    "publicKey b A = publicKey c A' ==> b=c & A=A'"
 
-use "Public_lemmas.ML"
+  (*No private key equals any public key (essential to ensure that private
+    keys are private!) *)
+  privateKey_neq_publicKey [iff]: "privateKey b A \<noteq> publicKey c A'"
 
-lemma [simp]: "K \\<in> symKeys ==> invKey K = K"
+
+
+
+(*** Basic properties of pubK & priK ***)
+
+lemma [iff]: "(publicKey b A = publicKey c A') = (b=c & A=A')"
+by (blast dest!: injective_publicKey) 
+
+lemma [iff]:
+    "(privateKey b A = privateKey c A') = (b=c & A=A')"
+apply (rule iffI) 
+apply (drule_tac f = "invKey" in arg_cong)
+apply (auto ); 
+done
+
+declare privateKey_neq_publicKey [THEN not_sym, iff]
+
+lemma not_symKeys_pubK [iff]: "publicKey b A \<notin> symKeys"
+apply (simp add: symKeys_def)
+done
+
+lemma not_symKeys_priK [iff]: "privateKey b A \<notin> symKeys"
+apply (simp add: symKeys_def)
+done
+
+lemma symKey_neq_priEK: "K \<in> symKeys ==> K \<noteq> priEK A"
+by auto
+
+lemma symKeys_neq_imp_neq: "(K \<in> symKeys) \<noteq> (K' \<in> symKeys) ==> K \<noteq> K'"
+apply blast
+done
+
+lemma symKeys_invKey_iff [iff]: "(invKey K \<in> symKeys) = (K \<in> symKeys)"
+apply (unfold symKeys_def)
+apply auto
+done
+
+lemma analz_symKeys_Decrypt:
+     "[| Crypt K X \<in> analz H;  K \<in> symKeys;  Key K \<in> analz H |]  
+      ==> X \<in> analz H"
+by (auto simp add: symKeys_def)
+
+
+
+subsection{*"Image" equations that hold for injective functions*}
+
+lemma invKey_image_eq [simp]: "(invKey x \<in> invKey`A) = (x \<in> A)"
+apply auto
+done
+
+(*holds because invKey is injective*)
+lemma publicKey_image_eq [simp]:
+     "(publicKey b x \<in> publicKey c ` AA) = (b=c & x \<in> AA)"
+by auto
+
+lemma privateKey_notin_image_publicKey [simp]: "privateKey b x \<notin> publicKey c ` AA"
+apply auto
+done
+
+lemma privateKey_image_eq [simp]:
+     "(privateKey b A \<in> invKey ` publicKey c ` AS) = (b=c & A\<in>AS)"
+by auto
+
+lemma publicKey_notin_image_privateKey [simp]: "publicKey b A \<notin> invKey ` publicKey c ` AS"
+apply auto
+done
+
+
+subsection{*Symmetric Keys*}
+
+text{*For some protocols, it is convenient to equip agents with symmetric as
+well as asymmetric keys.  The theory @{text Shared} assumes that all keys
+are symmetric.*}
+
+consts
+  shrK    :: "agent => key"    --{*long-term shared keys*}
+
+axioms
+  inj_shrK: "inj shrK"	             --{*No two agents have the same key*}
+  sym_shrK [iff]: "shrK X \<in> symKeys" --{*All shared keys are symmetric*}
+
+(*Injectiveness: Agents' long-term keys are distinct.*)
+declare inj_shrK [THEN inj_eq, iff]
+
+lemma priK_neq_shrK [iff]: "shrK A \<noteq> privateKey b C"
+apply (simp add: symKeys_neq_imp_neq)
+done
+
+declare priK_neq_shrK [THEN not_sym, simp]
+
+lemma pubK_neq_shrK [iff]: "shrK A \<noteq> publicKey b C"
+apply (simp add: symKeys_neq_imp_neq)
+done
+
+declare pubK_neq_shrK [THEN not_sym, simp]
+
+lemma priEK_noteq_shrK [simp]: "priEK A \<noteq> shrK B" 
+by auto
+
+lemma publicKey_notin_image_shrK [simp]: "publicKey b x \<notin> shrK ` AA"
+by auto
+
+lemma privateKey_notin_image_shrK [simp]: "privateKey b x \<notin> shrK ` AA"
+by auto
+
+lemma shrK_notin_image_publicKey [simp]: "shrK x \<notin> publicKey b ` AA"
+by auto
+
+lemma shrK_notin_image_privateKey [simp]: "shrK x \<notin> invKey ` publicKey b ` AA" 
+by auto
+
+lemma shrK_image_eq [simp]: "(shrK x \<in> shrK ` AA) = (x \<in> AA)"
+by auto
+
+
+subsection{*Initial States of Agents*}
+
+text{*Note: for all practical purposes, all that matters is the initial
+knowledge of the Spy.  All other agents are automata, merely following the
+protocol.*}
+
+primrec
+        (*Agents know their private key and all public keys*)
+  initState_Server:
+    "initState Server     =    
+       {Key (priEK Server), Key (priSK Server)} \<union> 
+       (Key ` range pubEK) \<union> (Key ` range pubSK) \<union> (Key ` range shrK)"
+
+  initState_Friend:
+    "initState (Friend i) =    
+       {Key (priEK(Friend i)), Key (priSK(Friend i)), Key (shrK(Friend i))} \<union> 
+       (Key ` range pubEK) \<union> (Key ` range pubSK)"
+
+  initState_Spy:
+    "initState Spy        =    
+       (Key ` invKey ` pubEK ` bad) \<union> (Key ` invKey ` pubSK ` bad) \<union> 
+       (Key ` shrK ` bad) \<union> 
+       (Key ` range pubEK) \<union> (Key ` range pubSK)"
+
+
+
+text{*These lemmas allow reasoning about @{term "used evs"} rather than
+   @{term "knows Spy evs"}, which is useful when there are private Notes. *}
+
+lemma used_parts_subset_parts [rule_format]:
+     "\<forall>X \<in> used evs. parts {X} \<subseteq> used evs"
+apply (induct evs) 
+ prefer 2
+ apply (simp add: used_Cons)
+ apply (rule ballI)  
+ apply (case_tac a, auto)
+ apply (drule parts_cut, assumption, simp) 
+ apply (drule parts_cut, assumption, simp) 
+txt{*Base case*}
+apply (simp add: used_Nil, clarify) 
+apply (rename_tac B) 
+apply (rule_tac x=B in exI) 
+apply (case_tac B, auto) 
+done
+
+lemma MPair_used_D: "{|X,Y|} \<in> used H ==> X \<in> used H & Y \<in> used H"
+by (drule used_parts_subset_parts, simp, blast)
+
+lemma MPair_used [elim!]:
+     "[| {|X,Y|} \<in> used H;
+         [| X \<in> used H; Y \<in> used H |] ==> P |] 
+      ==> P"
+by (blast dest: MPair_used_D) 
+
+
+text{*Rewrites should not refer to  @{term "initState(Friend i)"} because
+  that expression is not in normal form.*}
+
+lemma keysFor_parts_initState [simp]: "keysFor (parts (initState C)) = {}"
+apply (unfold keysFor_def)
+apply (induct_tac "C")
+apply (auto intro: range_eqI)
+done
+
+lemma Crypt_notin_initState: "Crypt K X \<notin> parts (initState B)"
+by (induct B, auto)
+
+
+(*** Basic properties of shrK ***)
+
+(*Agents see their own shared keys!*)
+lemma shrK_in_initState [iff]: "Key (shrK A) \<in> initState A"
+apply (induct_tac "A")
+apply auto
+done
+
+lemma shrK_in_knows [iff]: "Key (shrK A) \<in> knows A evs"
+by (simp add: initState_subset_knows [THEN subsetD])
+
+lemma shrK_in_used [iff]: "Key (shrK A) \<in> used evs"
+apply (rule initState_into_used)
+apply blast
+done
+
+(** Fresh keys never clash with long-term shared keys **)
+
+(*Used in parts_induct_tac and analz_Fake_tac to distinguish session keys
+  from long-term shared keys*)
+lemma Key_not_used: "Key K \<notin> used evs ==> K \<notin> range shrK"
+apply blast
+done
+
+lemma shrK_neq: "Key K \<notin> used evs ==> shrK B \<noteq> K"
+apply blast
+done
+
+
+
+subsection{*Function @{term spies} *}
+
+text{*Agents see their own private keys!*}
+lemma priK_in_initState [iff]: "Key (privateKey b A) \<in> initState A"
+apply (induct_tac "A")
+apply auto
+done
+
+text{*Agents see all public keys!*}
+lemma publicKey_in_initState [iff]: "Key (publicKey b A) \<in> initState B"
+apply (case_tac "B")
+apply auto
+done
+
+text{*All public keys are visible*}
+lemma spies_pubK [iff]: "Key (publicKey b A) \<in> spies evs"
+apply (induct_tac "evs")
+apply (simp_all add: imageI knows_Cons split add: event.split)
+done
+
+declare spies_pubK [THEN analz.Inj, iff]
+
+text{*Spy sees private keys of bad agents!*}
+lemma Spy_spies_bad_privateKey [intro!]:
+     "A \<in> bad ==> Key (privateKey b A) \<in> spies evs"
+apply (induct_tac "evs")
+apply (simp_all add: imageI knows_Cons split add: event.split)
+done
+
+text{*Spy sees long-term shared keys of bad agents!*}
+lemma Spy_spies_bad_shrK [intro!]:
+     "A \<in> bad ==> Key (shrK A) \<in> spies evs"
+apply (induct_tac "evs")
+apply (simp_all add: imageI knows_Cons split add: event.split)
+done
+
+lemma publicKey_into_used [iff] :"Key (publicKey b A) \<in> used evs"
+apply (rule initState_into_used)
+apply (rule publicKey_in_initState [THEN parts.Inj])
+done
+
+lemma privateKey_into_used [iff]: "Key (privateKey b A) \<in> used evs"
+apply(rule initState_into_used)
+apply(rule priK_in_initState [THEN parts.Inj])
+done
+
+
+subsection{*Fresh Nonces*}
+
+lemma Nonce_notin_initState [iff]: "Nonce N \<notin> parts (initState B)"
+apply (induct_tac "B")
+apply auto
+done
+
+lemma Nonce_notin_used_empty [simp]: "Nonce N \<notin> used []"
+apply (simp add: used_Nil)
+done
+
+
+subsection{*Supply fresh nonces for possibility theorems*}
+
+text{*In any trace, there is an upper bound N on the greatest nonce in use*}
+lemma Nonce_supply_lemma: "EX N. ALL n. N<=n --> Nonce n \<notin> used evs"
+apply (induct_tac "evs")
+apply (rule_tac x = "0" in exI)
+apply (simp_all (no_asm_simp) add: used_Cons split add: event.split)
+apply safe
+apply (rule msg_Nonce_supply [THEN exE], blast elim!: add_leE)+
+done
+
+lemma Nonce_supply1: "EX N. Nonce N \<notin> used evs"
+apply (rule Nonce_supply_lemma [THEN exE])
+apply blast
+done
+
+lemma Nonce_supply: "Nonce (@ N. Nonce N \<notin> used evs) \<notin> used evs"
+apply (rule Nonce_supply_lemma [THEN exE])
+apply (rule someI)
+apply fast
+done
+
+subsection{*Specialized rewriting for the analz_image_... theorems*}
+
+lemma insert_Key_singleton: "insert (Key K) H = Key ` {K} Un H"
+apply blast
+done
+
+lemma insert_Key_image: "insert (Key K) (Key`KK \<union> C) = Key ` (insert K KK) \<union> C"
+apply blast
+done
+
+ML
+{*
+val Key_not_used = thm "Key_not_used";
+val insert_Key_singleton = thm "insert_Key_singleton";
+val insert_Key_image = thm "insert_Key_image";
+*}
+
+(*
+val not_symKeys_pubK = thm "not_symKeys_pubK";
+val not_symKeys_priK = thm "not_symKeys_priK";
+val symKeys_neq_imp_neq = thm "symKeys_neq_imp_neq";
+val analz_symKeys_Decrypt = thm "analz_symKeys_Decrypt";
+val invKey_image_eq = thm "invKey_image_eq";
+val pubK_image_eq = thm "pubK_image_eq";
+val priK_pubK_image_eq = thm "priK_pubK_image_eq";
+val keysFor_parts_initState = thm "keysFor_parts_initState";
+val priK_in_initState = thm "priK_in_initState";
+val spies_pubK = thm "spies_pubK";
+val Spy_spies_bad = thm "Spy_spies_bad";
+val Nonce_notin_initState = thm "Nonce_notin_initState";
+val Nonce_notin_used_empty = thm "Nonce_notin_used_empty";
+
+*)
+
+
+lemma invKey_K [simp]: "K \<in> symKeys ==> invKey K = K"
 by (simp add: symKeys_def)
 
-(*Specialized methods*)
+lemma Crypt_imp_keysFor :"[|K \<in> symKeys; Crypt K X \<in> H|] ==> K \<in> keysFor H"
+apply (drule Crypt_imp_invKey_keysFor, simp)
+done
+
+
+subsection{*Specialized Methods for Possibility Theorems*}
+
+ML
+{*
+val Nonce_supply1 = thm "Nonce_supply1";
+val Nonce_supply = thm "Nonce_supply";
+
+(*Tactic for possibility theorems (Isar interface)*)
+fun gen_possibility_tac ss state = state |>
+    REPEAT (*omit used_Says so that Nonces start from different traces!*)
+    (ALLGOALS (simp_tac (ss delsimps [used_Says]))
+     THEN
+     REPEAT_FIRST (eq_assume_tac ORELSE' 
+                   resolve_tac [refl, conjI, Nonce_supply]))
+
+(*Tactic for possibility theorems (ML script version)*)
+fun possibility_tac state = gen_possibility_tac (simpset()) state
+*}
 
 method_setup possibility = {*
     Method.ctxt_args (fn ctxt =>
         Method.METHOD (fn facts =>
             gen_possibility_tac (Simplifier.get_local_simpset ctxt))) *}
     "for proving possibility theorems"
+
+
+
+ML
+{*
+bind_thms ("analz_image_freshK_simps",
+           simp_thms @ mem_simps @  (*these two allow its use with only:*)
+           disj_comms @
+           [image_insert RS sym, image_Un RS sym, empty_subsetI, insert_subset,
+            analz_insert_eq, impOfSubs (Un_upper2 RS analz_mono),
+	    insert_Key_singleton, 
+            Key_not_used, insert_Key_image, Un_assoc RS sym]);
+
+val analz_image_freshK_ss =
+     simpset() delsimps [image_insert, image_Un]
+	       delsimps [imp_disjL]    (*reduces blow-up*)
+	       addsimps analz_image_freshK_simps;
+*}
 
 end
